Very messy snapshot of work adding IfEqual; had to mark a hint in Buffers as local and compensate elsewhere

platform/XmlOutput.v
@@ -1,5 +1,10 @@
-Require Import AutoSep Wrap StringOps XmlLex SinglyLinkedList Malloc ArrayOps Bags.
+Require Import AutoSep Wrap StringOps SinglyLinkedList Malloc ArrayOps Bags.
 Require Import RelDb RelDbCondition RelDbSelect.
+Print HintDb core.
+
+Require Import RelDb RelDbCondition RelDbSelect.
+Print HintDb core.
+
 
 Set Implicit Arguments.
 
@@ -10,8 +15,9 @@ Inductive xml :=
 | Cdata (const : string)
 | Var (start len : string)
 | Tag (tag : string) (inner : list xml)
-| Column (data : string) (col : string)
-| Select (tab rw data : string) (cond : condition) (inner : xml).
+| Column (tab : string) (col : string)
+| Select (tab rw data : string) (cond : condition) (inner : xml)
+| IfEqual (tab1 col1 tab2 col2 : string) (inner : xml).
 
 Section ForallR.
   Variable A : Type.
@@ -82,7 +88,8 @@ Fixpoint removeTable (tab : string) (ts : tables) : tables :=
   end.
 
 Definition cvars := "rp" :: "ibuf" :: "overflowed" :: "ipos" :: "ilen"
-  :: "opos" :: "tmp" :: "len" :: "buf":: "matched" :: "res" :: "obuf" :: "olen" :: nil.
+  :: "opos" :: "tmp" :: "len" :: "buf" :: "matched" :: "res" :: "obuf"
+  :: "olen" :: nil.
 
 Definition dontTouch rw data :=
   ForallR (fun p : string * string => fst p <> rw /\ snd p <> rw /\ fst p <> data /\ snd p <> data).
@@ -103,6 +110,14 @@ Fixpoint wf ns (cdatas : list (string * string)) (avs : list avail) (ts : list t
       /\ exists t, In t ts /\ Name t = tab /\ cwf ns (Schema t) cdatas cond
         /\ wf ns cdatas ({| Table := t; Row := rw; Data := data |} :: avs)
         (removeTable tab ts) inner
+    | IfEqual tab1 col1 tab2 col2 inner => tab1 <> tab2
+      /\ (exists av, In av avs /\ Name (Table av) = tab1
+        /\ In col1 (Schema (Table av))
+        /\ In (Data av) ns)
+      /\ (exists av, In av avs /\ Name (Table av) = tab2
+        /\ In col2 (Schema (Table av))
+        /\ In (Data av) ns)
+      /\ wf ns cdatas avs ts inner
   end.
 
 
@@ -120,6 +135,7 @@ Fixpoint freeVar (xm : xml) (xs : string * string) : Prop :=
     | Column _ _ => False
     | Select _ _ _ cond inner => List.Exists (fun e => efreeVar (snd e) xs) cond
       \/ freeVar inner xs
+    | IfEqual _ _ _ _ inner => freeVar inner xs
   end.
 
 Fixpoint bindsRowVar (xm : xml) (xs : string * string) : Prop :=
@@ -129,6 +145,7 @@ Fixpoint bindsRowVar (xm : xml) (xs : string * string) : Prop :=
     | Tag _ inner => ExistsR (fun xm' => bindsRowVar xm' xs) inner
     | Column _ _ => False
     | Select _ rw data _ inner => xs = (rw, data) \/ bindsRowVar inner xs
+    | IfEqual _ _ _ _ inner => bindsRowVar inner xs
   end.
 
 Section xml_ind'.
@@ -145,6 +162,9 @@ Section xml_ind'.
   Hypothesis H_Select : forall tab rw data cond inner, P inner
     -> P (Select tab rw data cond inner).
 
+  Hypothesis H_IfEqual : forall tab1 col1 tab2 col2 inner, P inner
+    -> P (IfEqual tab1 col1 tab2 col2 inner).
+
   Fixpoint xml_ind' (xm : xml) : P xm :=
     match xm with
       | Cdata const => H_Cdata const
@@ -155,7 +175,10 @@ Section xml_ind'.
           | xm :: xms' => Forall_cons _ (xml_ind' xm) (xmls_ind xms')
         end) inner)
       | Column tab col => H_Column tab col
-      | Select tab rw data cond inner => H_Select tab rw data cond (xml_ind' inner)
+      | Select tab rw data cond inner =>
+        H_Select tab rw data cond (xml_ind' inner)
+      | IfEqual tab1 col1 tab2 col2 inner =>
+        H_IfEqual tab1 col1 tab2 col2 (xml_ind' inner)
     end.
 End xml_ind'.
 
@@ -269,7 +292,8 @@ Definition cdatasGood (cdatas : list (string * string)) :=
   List.Forall (fun p => fst p <> "opos" /\ fst p <> "overflowed" /\ fst p <> "tmp" /\ fst p <> "matched"
     /\ fst p <> "res" /\ fst p <> "ibuf" /\ fst p <> "ilen" /\ fst p <> "ipos"
     /\ snd p <> "opos" /\ snd p <> "overflowed" /\ snd p <> "tmp" /\ snd p <> "matched"
-    /\ snd p <> "res" /\ snd p <> "ibuf" /\ snd p <> "ilen" /\ snd p <> "ipos") cdatas.
+    /\ snd p <> "res" /\ snd p <> "ibuf" /\ snd p <> "ilen" /\ snd p <> "ipos")
+  cdatas.
 
 Lemma removeTable_bwd' : forall x ts P,
   NoDup (Names ts)
@@ -511,7 +535,7 @@ Lemma findCol_lenl : forall sch col cols,
   intros; rewrite length_lenl; eauto using findCol_bound_natToW.
 Qed.
 
-Hint Immediate findCol_posl findCol_lenl.
+Hint Resolve findCol_posl findCol_lenl.
 
 Lemma selN_col : forall sch col cols,
   In col sch
@@ -560,8 +584,8 @@ Hint Extern 1 (_ + _ <= _)%nat =>
 
 Lemma findCursor_good : forall tab av avs,
   NoDup (map (fun av => Name (Table av)) avs)
-  -> In av avs
   -> Name (Table av) = tab
+  -> In av avs
   -> findCursor tab avs = Some av.
   induction avs; simpl; inversion 1; intuition subst; ift.
   exfalso; eapply H2.
@@ -792,6 +816,29 @@ Qed.
 
 Hint Immediate NoDups_move.
 
+Check toCmd.
+
+Module Type TO_CMD.
+  Parameter toCmd' : chunk ->
+    forall (im : LabelMap.t assert) (mn : string),
+      importsGlobal im -> list string -> nat -> cmd im mn.
+
+  Axiom toCmd'_eq : toCmd' = toCmd.
+End TO_CMD.
+
+Module ToCmd : TO_CMD.
+  Definition toCmd' := toCmd.
+
+  Theorem toCmd'_eq : toCmd' = toCmd.
+    auto.
+  Qed.
+End ToCmd.
+
+Import ToCmd.
+
+Definition clarify (ch : chunk) : chunk := fun ns n =>
+  Structured nil (fun im mn H => toCmd' ch mn H ns n).
+
 
 (** * Compiling XML snippets into Bedrock chunks *)
 
@@ -983,6 +1030,307 @@ Section Out.
               (removeTable tab ts)
               inner)
         end
+
+      | IfEqual tab1 col1 tab2 col2 inner =>
+        match findCursor tab1 avs, findCursor tab2 avs with
+          | Some av1, Some av2 =>
+            If ("overflowed" = 0) {
+              Assert [Al a : A, Al bsI, Al bsO,
+                PRE[V] array8 bsI (V "buf") * array8 bsO (V "obuf")
+                  * [| length bsI = wordToNat (V "len") |]
+                  * [| length bsO = wordToNat (V "olen") |]
+                  * [| inBounds cdatas V |] * [| V "opos" <= V "olen" |]%word
+                  * cursor V av1 * cursor V av2
+                  * cursors V (removeCursor tab2 (removeCursor tab1 avs))
+                  * db ts * invPre a V
+                POST[R] Ex bsO', array8 bsI (V "buf") * array8 bsO' (V "obuf")
+                  * [| length bsO' = length bsO |] * invPost a V R];;
+
+              Note [reveal_row];;
+
+              Assert [Al a : A, Al bsI, Al bsO,
+                PRE[V] array8 bsI (V "buf") * array8 bsO (V "obuf")
+                  * [| length bsI = wordToNat (V "len") |]
+                  * [| length bsO = wordToNat (V "olen") |]
+                  * [| inBounds cdatas V |] * [| V "opos" <= V "olen" |]%word
+                  * invPre a V
+                  * cursors V (removeCursor tab2 (removeCursor tab1 avs)) * db ts
+                  * RelDbSelect.inv (Address (Table av1)) (Schema (Table av1))
+                  (V (Row av1)) (V (Data av1))
+                  * RelDbSelect.inv (Address (Table av2)) (Schema (Table av2))
+                  (V (Row av2)) (V (Data av2))
+                  * (Ex buf1, Ex len1, Ex cols1, Ex bs1,
+                    (V (Data av1) ==*> buf1, len1)
+                    * array (posl cols1) (V (Data av1) ^+ $8)
+                    * array (lenl cols1) (V (Data av1) ^+ $8
+                      ^+ $(length (Schema (Table av1)) * 4)) * array8 bs1 buf1
+                    * [| length bs1 = wordToNat len1 |]
+                    * [| length cols1 = length (Schema (Table av1)) |]
+                    * [| RelDb.inBounds len1 cols1 |]
+                    * [| V (Data av1) <> 0 |]
+                    * [| freeable (V (Data av1))
+                      (2 + length (Schema (Table av1))
+                        + length (Schema (Table av1))) |]
+                    * [| buf1 <> 0 |] * [| freeable8 buf1 (length bs1) |]
+                    * [| natToW (findCol (Schema (Table av1)) col1)
+                      < natToW (length (lenl cols1)) |]%word)
+                  * (Ex buf2, Ex len2, Ex cols2, Ex bs2,
+                    (V (Data av2) ==*> buf2, len2)
+                    * array (posl cols2) (V (Data av2) ^+ $8)
+                    * array (lenl cols2) (V (Data av2) ^+ $8
+                      ^+ $(length (Schema (Table av2)) * 4)) * array8 bs2 buf2
+                    * [| length bs2 = wordToNat len2 |]
+                    * [| length cols2 = length (Schema (Table av2)) |]
+                    * [| RelDb.inBounds len2 cols2 |]
+                    * [| V (Data av2) <> 0 |]
+                    * [| freeable (V (Data av2))
+                      (2 + length (Schema (Table av2))
+                        + length (Schema (Table av2))) |]
+                    * [| buf2 <> 0 |] * [| freeable8 buf2 (length bs2) |]
+                    * [| natToW (findCol (Schema (Table av2)) col2)
+                      < natToW (length (lenl cols2)) |]%word)
+                POST[R] Ex bsO', array8 bsI (V "buf") * array8 bsO' (V "obuf")
+                  * [| length bsO' = length bsO |] * invPost a V R];;
+
+              "matched" <- Data av1 + 8;;
+              "matched" <- "matched" + (length (Schema (Table av1)) * 4)%nat;;
+              "matched" <-* "matched" + (4 * findCol (Schema (Table av1)) col1)%nat;;
+
+              Assert [Al a : A, Al bsI, Al bsO,
+                PRE[V] array8 bsI (V "buf") * array8 bsO (V "obuf")
+                  * [| length bsI = wordToNat (V "len") |]
+                  * [| length bsO = wordToNat (V "olen") |]
+                  * [| inBounds cdatas V |] * [| V "opos" <= V "olen" |]%word
+                  * invPre a V
+                  * cursors V (removeCursor tab2 (removeCursor tab1 avs)) * db ts
+                  * RelDbSelect.inv (Address (Table av1)) (Schema (Table av1))
+                  (V (Row av1)) (V (Data av1))
+                  * RelDbSelect.inv (Address (Table av2)) (Schema (Table av2))
+                  (V (Row av2)) (V (Data av2))
+                  * (Ex buf1, Ex len1, Ex cols1, Ex bs1,
+                    (V (Data av1) ==*> buf1, len1)
+                    * array (posl cols1) (V (Data av1) ^+ $8)
+                    * array (lenl cols1) (V (Data av1) ^+ $8
+                      ^+ $(length (Schema (Table av1)) * 4)) * array8 bs1 buf1
+                    * [| length bs1 = wordToNat len1 |]
+                    * [| length cols1 = length (Schema (Table av1)) |]
+                    * [| RelDb.inBounds len1 cols1 |]
+                    * [| V (Data av1) <> 0 |]
+                    * [| freeable (V (Data av1))
+                      (2 + length (Schema (Table av1))
+                        + length (Schema (Table av1))) |]
+                    * [| buf1 <> 0 |] * [| freeable8 buf1 (length bs1) |]
+                    * [| V "matched" = Array.selN (lenl cols1)
+                        (findCol (Schema (Table av1)) col1) |])
+                  * (Ex buf2, Ex len2, Ex cols2, Ex bs2,
+                    (V (Data av2) ==*> buf2, len2)
+                    * array (posl cols2) (V (Data av2) ^+ $8)
+                    * array (lenl cols2) (V (Data av2) ^+ $8
+                      ^+ $(length (Schema (Table av2)) * 4)) * array8 bs2 buf2
+                    * [| length bs2 = wordToNat len2 |]
+                    * [| length cols2 = length (Schema (Table av2)) |]
+                    * [| RelDb.inBounds len2 cols2 |]
+                    * [| V (Data av2) <> 0 |]
+                    * [| freeable (V (Data av2))
+                      (2 + length (Schema (Table av2))
+                        + length (Schema (Table av2))) |]
+                    * [| buf2 <> 0 |] * [| freeable8 buf2 (length bs2) |]
+                    * [| natToW (findCol (Schema (Table av2)) col2)
+                      < natToW (length (lenl cols2)) |]%word)
+                POST[R] Ex bsO', array8 bsI (V "buf") * array8 bsO' (V "obuf")
+                  * [| length bsO' = length bsO |] * invPost a V R];;
+
+              "tmp" <- Data av2 + 8;;
+              "tmp" <- "tmp" + (length (Schema (Table av2)) * 4)%nat;;
+              "tmp" <-* "tmp" + (4 * findCol (Schema (Table av2)) col2)%nat;;
+
+              "tmp" <- "olen" - "opos";;
+              Note [reveal_row];;
+              If ("matched" = "tmp") {
+                Assert [Al a : A, Al bsI, Al bsO,
+                  PRE[V] array8 bsI (V "buf") * array8 bsO (V "obuf")
+                    * [| length bsI = wordToNat (V "len") |]
+                    * [| length bsO = wordToNat (V "olen") |]
+                    * [| inBounds cdatas V |] * [| V "opos" <= V "olen" |]%word
+                    * invPre a V
+                    * cursors V (removeCursor tab2 (removeCursor tab1 avs))
+                    * db ts
+                    * RelDbSelect.inv (Address (Table av1)) (Schema (Table av1))
+                    (V (Row av1)) (V (Data av1))
+                    * RelDbSelect.inv (Address (Table av2)) (Schema (Table av2))
+                    (V (Row av2)) (V (Data av2))
+                    * (Ex buf1, Ex len1, Ex cols1, Ex bs1,
+                      (V (Data av1) ==*> buf1, len1)
+                      * array (posl cols1) (V (Data av1) ^+ $8)
+                      * array (lenl cols1) (V (Data av1) ^+ $8
+                        ^+ $(length (Schema (Table av1)) * 4)) * array8 bs1 buf1
+                      * [| length bs1 = wordToNat len1 |]
+                      * [| length cols1 = length (Schema (Table av1)) |]
+                      * [| RelDb.inBounds len1 cols1 |]
+                      * [| V (Data av1) <> 0 |]
+                      * [| freeable (V (Data av1)) (2
+                        + length (Schema (Table av1))
+                        + length (Schema (Table av1))) |]
+                      * [| buf1 <> 0 |] * [| freeable8 buf1 (length bs1) |]
+                      * [| V "matched" = Array.selN (lenl cols1)
+                        (findCol (Schema (Table av1)) col1) |]
+                      * [| natToW (findCol (Schema (Table av1)) col1)
+                        < natToW (length (posl cols1)) |]%word)
+                    * (Ex buf2, Ex len2, Ex cols2, Ex bs2,
+                      (V (Data av2) ==*> buf2, len2)
+                      * array (posl cols2) (V (Data av2) ^+ $8)
+                      * array (lenl cols2) (V (Data av2) ^+ $8
+                        ^+ $(length (Schema (Table av2)) * 4)) * array8 bs2 buf2
+                      * [| length bs2 = wordToNat len2 |]
+                      * [| length cols2 = length (Schema (Table av2)) |]
+                      * [| RelDb.inBounds len2 cols2 |]
+                      * [| V (Data av2) <> 0 |]
+                      * [| freeable (V (Data av2)) (2
+                        + length (Schema (Table av2))
+                        + length (Schema (Table av2))) |]
+                      * [| buf2 <> 0 |] * [| freeable8 buf2 (length bs2) |]
+                      * [| V "tmp" = Array.selN (lenl cols2)
+                        (findCol (Schema (Table av2)) col2) |]
+                      * [| natToW (findCol (Schema (Table av2)) col2)
+                        < natToW (length (posl cols2)) |]%word)
+                    * [| V "matched" = V "tmp" |]%word
+                  POST[R] Ex bsO', array8 bsI (V "buf") * array8 bsO' (V "obuf")
+                    * [| length bsO' = length bsO |] * invPost a V R];;
+
+                "tmp" <- Data av1 + 8;;
+                "tmp" <-* "tmp" + (4 * findCol (Schema (Table av1)) col1)%nat;;
+
+                Assert [Al a : A, Al bsI, Al bsO,
+                  PRE[V] array8 bsI (V "buf") * array8 bsO (V "obuf")
+                    * [| length bsI = wordToNat (V "len") |]
+                    * [| length bsO = wordToNat (V "olen") |]
+                    * [| inBounds cdatas V |] * [| V "opos" <= V "olen" |]%word
+                    * invPre a V
+                    * cursors V (removeCursor tab2 (removeCursor tab1 avs))
+                    * db ts
+                    * RelDbSelect.inv (Address (Table av1)) (Schema (Table av1))
+                    (V (Row av1)) (V (Data av1))
+                    * RelDbSelect.inv (Address (Table av2)) (Schema (Table av2))
+                    (V (Row av2)) (V (Data av2))
+                    * (Ex buf1, Ex len1, Ex cols1, Ex bs1,
+                      (V (Data av1) ==*> buf1, len1)
+                      * array (posl cols1) (V (Data av1) ^+ $8)
+                      * array (lenl cols1) (V (Data av1) ^+ $8
+                        ^+ $(length (Schema (Table av1)) * 4)) * array8 bs1 buf1
+                      * [| length bs1 = wordToNat len1 |]
+                      * [| length cols1 = length (Schema (Table av1)) |]
+                      * [| RelDb.inBounds len1 cols1 |]
+                      * [| V (Data av1) <> 0 |]
+                      * [| freeable (V (Data av1)) (2
+                        + length (Schema (Table av1))
+                        + length (Schema (Table av1))) |]
+                      * [| buf1 <> 0 |] * [| freeable8 buf1 (length bs1) |]
+                      * [| V "matched" = Array.selN (lenl cols1)
+                        (findCol (Schema (Table av1)) col1) |]
+                      * [| V "tmp" = Array.selN (posl cols1)
+                        (findCol (Schema (Table av1)) col1) |])
+                    * (Ex buf2, Ex len2, Ex cols2, Ex bs2,
+                      (V (Data av2) ==*> buf2, len2)
+                      * array (posl cols2) (V (Data av2) ^+ $8)
+                      * array (lenl cols2) (V (Data av2) ^+ $8
+                        ^+ $(length (Schema (Table av2)) * 4)) * array8 bs2 buf2
+                      * [| length bs2 = wordToNat len2 |]
+                      * [| length cols2 = length (Schema (Table av2)) |]
+                      * [| RelDb.inBounds len2 cols2 |]
+                      * [| V (Data av2) <> 0 |]
+                      * [| freeable (V (Data av2)) (2
+                        + length (Schema (Table av2))
+                        + length (Schema (Table av2))) |]
+                      * [| buf2 <> 0 |] * [| freeable8 buf2 (length bs2) |]
+                      * [| V "tmp" = Array.selN (lenl cols2)
+                        (findCol (Schema (Table av2)) col2) |]
+                      * [| natToW (findCol (Schema (Table av2)) col2)
+                        < natToW (length (posl cols2)) |]%word)
+                    * [| V "matched" = V "tmp" |]%word
+                  POST[R] Ex bsO', array8 bsI (V "buf") * array8 bsO' (V "obuf")
+                    * [| length bsO' = length bsO |] * invPost a V R];;
+
+                "res" <- Data av2 + 8;;
+                "res" <-* "res" + (4 * findCol (Schema (Table av2)) col2)%nat;;
+
+                Note [reveal_row];;
+
+                Assert [Al a : A, Al bsI, Al bsO,
+                  PRE[V] array8 bsI (V "buf") * array8 bsO (V "obuf")
+                    * [| length bsI = wordToNat (V "len") |]
+                    * [| length bsO = wordToNat (V "olen") |]
+                    * [| inBounds cdatas V |] * [| V "opos" <= V "olen" |]%word
+                    * invPre a V
+                    * cursors V (removeCursor tab2 (removeCursor tab1 avs)) * db ts
+                    * RelDbSelect.inv (Address (Table av1)) (Schema (Table av1))
+                    (V (Row av1)) (V (Data av1))
+                    * RelDbSelect.inv (Address (Table av2)) (Schema (Table av2))
+                    (V (Row av2)) (V (Data av2))
+                    * (Ex buf1, Ex len1, Ex cols1, Ex bs1,
+                      (V (Data av1) ==*> buf1, len1)
+                      * array (posl cols1) (V (Data av1) ^+ $8)
+                      * array (lenl cols1) (V (Data av1) ^+ $8
+                        ^+ $(length (Schema (Table av1)) * 4)) * array8 bs1 buf1
+                      * [| length bs1 = wordToNat len1 |]
+                      * [| length cols1 = length (Schema (Table av1)) |]
+                      * [| RelDb.inBounds len1 cols1 |]
+                      * [| V (Data av1) <> 0 |]
+                      * [| freeable (V (Data av1)) (2
+                        + length (Schema (Table av1))
+                        + length (Schema (Table av1))) |]
+                      * [| buf1 <> 0 |] * [| freeable8 buf1 (length bs1) |]
+                      * [| V "matched" = Array.selN (lenl cols1)
+                        (findCol (Schema (Table av1)) col1) |]
+                      * [| V "tmp" = Array.selN (posl cols1)
+                        (findCol (Schema (Table av1)) col1) |])
+                    * (Ex buf2, Ex len2, Ex cols2, Ex bs2,
+                      (V (Data av2) ==*> buf2, len2)
+                      * array (posl cols2) (V (Data av2) ^+ $8)
+                      * array (lenl cols2) (V (Data av2) ^+ $8
+                        ^+ $(length (Schema (Table av2)) * 4)) * array8 bs2 buf2
+                      * [| length bs2 = wordToNat len2 |]
+                      * [| length cols2 = length (Schema (Table av2)) |]
+                      * [| RelDb.inBounds len2 cols2 |]
+                      * [| V (Data av2) <> 0 |]
+                      * [| freeable (V (Data av2)) (2
+                        + length (Schema (Table av2))
+                        + length (Schema (Table av2))) |]
+                      * [| buf2 <> 0 |] * [| freeable8 buf2 (length bs2) |]
+                      * [| V "matched" = Array.selN (lenl cols2)
+                        (findCol (Schema (Table av2)) col2) |]
+                      * [| V "res" = Array.selN (posl cols2)
+                        (findCol (Schema (Table av2)) col2) |])
+                  POST[R] Ex bsO', array8 bsI (V "buf") * array8 bsO' (V "obuf")
+                    * [| length bsO' = length bsO |] * invPost a V R];;
+
+                Note [reveal_row];;
+                "overflowed" <-* Data av1;;
+                Rp <-* Data av2;;
+
+                "res" <-- Call "array8"!"equal"("overflowed", "tmp", Rp, "res", "matched")
+                [Al a : A, Al bsI, Al bsO,
+                  PRE[V] array8 bsI (V "buf") * array8 bsO (V "obuf")
+                    * [| length bsI = wordToNat (V "len") |]
+                    * [| length bsO = wordToNat (V "olen") |]
+                    * [| inBounds cdatas V |] * [| V "opos" <= V "olen" |]%word
+                    * invPre a V * cursors V avs * db ts
+                  POST[R] Ex bsO', array8 bsI (V "buf")
+                    * array8 bsO' (V "obuf") * [| length bsO' = length bsO |]
+                    * invPost a V R];;
+
+                If ("res" = 1) {
+                  clarify (Out' cdatas avs ts inner)
+                } else {
+                  Skip
+                }
+              } else {
+                Note [reveal_row]
+              }
+            } else {
+              Skip
+            }
+          | _, _ => Fail
+        end
     end%SP.
 
   Opaque mult.
@@ -1019,6 +1367,11 @@ Section Out.
   Ltac reger := repeat match goal with
                          | [ H : Regs _ _ = _ |- _ ] => rewrite H
                        end.
+
+  Ltac my_refold :=
+    refold;
+    fold (@length B) in *; fold (@length string) in *;
+      fold (@length (W * W)) in *; fold (@length W) in *.
 
   Ltac simp :=
     repeat match goal with
@@ -1080,7 +1433,7 @@ Section Out.
                     evar (x : A); evar (y : B); let x' := eval unfold x in x in
                       let y' := eval unfold y in y in equate U (x', y'); clear x y; simpl
               end
-          end; autorewrite with sepFormula in *.
+          end; autorewrite with sepFormula in *; my_refold.
   
   Ltac deSpec :=
     repeat match goal with
@@ -1385,10 +1738,8 @@ Section Out.
           ZArith_dec.Z_ge_dec label'_eq label'_rec label'_rect COperand1 CTest
           COperand2 Pos.succ makeVcs Note_ Note__ IGotoStar_ IGotoStar
           AssertStar_ AssertStar Cond_ Cond
-          Wrap WrapC SimpleSeq StringWrite];
-        refold;
-        fold (@length B) in *; fold (@length string) in *;
-          fold (@length (W * W)) in *; fold (@length W) in *.
+          Wrap WrapC SimpleSeq StringWrite clarify];
+        my_refold.
 
     Ltac step1 :=
       match goal with
@@ -1429,6 +1780,59 @@ Section Out.
     Ltac step2 := abstract (deDouble; deSpec; intuition subst;
       solve [ t | proveHimp ]).
 
+    Lemma cursor_survived : forall tab t avs,
+      In t avs
+      -> tab <> Name (Table t)
+      -> In t (removeCursor tab avs).
+      clear; induction avs; simpl; intuition;
+        ift; simpl; intuition.
+    Qed.
+
+    Hint Immediate cursor_survived.
+
+    Lemma NoDup_survived' : forall tab' tab avs,
+      In tab' (ANames (removeCursor tab avs))
+      -> In tab' (ANames avs).
+      clear; induction avs; simpl; intuition;
+        generalize dependent H; ift; simpl in *; intuition.
+    Qed.
+
+    Lemma NoDup_survived : forall tab avs,
+      NoDup (ANames avs)
+      -> NoDup (ANames (removeCursor tab avs)).
+      clear; induction avs; inversion_clear 1; simpl; intuition.
+      ift; simpl; intuition eauto using NoDup_survived'.
+    Qed.
+
+    Hint Resolve NoDup_survived.
+
+    Lemma double_cursor_appear : forall V avs av1 av2 P,
+      In av1 avs
+      -> In av2 avs
+      -> Name (Table av1) <> Name (Table av2)
+      -> NoDup (ANames avs)
+      -> cursors V avs * P
+      ===> P * (cursor V av1 * (cursor V av2
+        * cursors V (removeCursor (Name (Table av2))
+          (removeCursor (Name (Table av1)) avs)))).
+      clear; sepLemma.
+      etransitivity; [ apply release_cursor; try apply H; eauto | ]; sepLemma.
+      etransitivity; [ apply release_cursor; eauto | ]; sepLemma.
+    Qed.
+
+    Hint Extern 1 (himp _ _ _) => apply double_cursor_appear.
+
+    Lemma goodSize_goodCursors : forall t avs,
+      In t avs
+      -> goodCursors avs
+      -> goodSize (length (Schema (Table t))).
+      clear; intros.
+      eapply Forall_forall in H0; [ | eassumption ].
+      tauto.
+    Qed.
+
+    Hint Immediate goodSize_goodCursors.
+
     Lemma Out_correct : forall cdatas, cdatasGood cdatas
       -> incl baseVars ns
       -> forall xm avs ts pre im mn (H : importsGlobal im),
@@ -1459,6 +1863,412 @@ Section Out.
           -> interp specs (invar cdatas avs ts true (fun x => x) ns res st))
         /\ vcs (VerifCond (toCmd (Out' cdatas avs ts xm) mn H ns res pre)).
       induction xm using xml_ind'.
+
+      Focus 6.
+      match goal with
+        | [ |- context[IfEqual] ] =>
+          simpl; propxFo;
+            do 2 erewrite findCursor_good in * by eauto(*;
+              try match goal with
+                    | [ H : interp _ _ |- _ ] =>
+                      generalize dependent H; vcgen_simp; propxFo
+                  end*)
+      end.
+
+      admit.
+      (*deDouble; intuition subst;
+        match goal with
+          | [ H : interp _ _ |- _ ] =>
+            rewrite toCmd'_eq in H;
+              apply IHxm in H; eauto; [ | clear H ]; (deSpec; t)
+        end.
+
+      step2.
+      step2.
+      step2.*)
+
+      vcgen_simp; wrap0.
+
+      admit. admit. admit. admit. admit. admit.
+      (*step2.
+      step2.
+      step2.
+      step2.
+      step2.
+      step2.*)
+
+      deDouble; deSpec; intuition subst.
+      post.
+      repeat invoke1.
+      prep.
+      propxFo.
+      repeat invoke1.
+      prepl.
+      evaluate auto_ext.
+
+      desc.
+      sep_canceller ltac:ILTacCommon.isConst auto_ext
+      ltac:(hints_ext_simplifier auto_ext).
+      (*sep_easy.*)
+      repeat
+        match goal with
+          | H:Logic.ex _ |- _ => destruct H
+          | H:_ /\ _ |- _ => destruct H
+          | |- Logic.ex _ => sep_easy; eexists
+          | |- _ /\ _ => split
+          | |- forall x, _ => intro
+          | |- _ = _ => reflexivity
+          | |- himp _ _ _ =>
+            reflexivity ||
+              (apply frame_reflexivity;
+                try match goal with
+                      | |- _ = ?X => instantiate ( 1 := X ) 
+                    end; apply eq_refl)
+        end.
+
+      sep_easy; autorewrite with sepFormula ; rereg; try subst.
+      2: sep_easy; autorewrite with sepFormula ; rereg; try subst.
+      3: sep_easy; autorewrite with sepFormula ; rereg; try subst.
+      3: sep_easy; autorewrite with sepFormula ; rereg; try subst.
+      3: sep_easy; autorewrite with sepFormula ; rereg; try subst.
+      4: sep_easy; autorewrite with sepFormula ; rereg; try subst.
+      5: sep_easy; autorewrite with sepFormula ; rereg; try subst.
+      6: sep_easy; autorewrite with sepFormula ; rereg; try subst.
+      7: sep_easy; autorewrite with sepFormula ; rereg; try subst.
+      8: sep_easy; autorewrite with sepFormula ; rereg; try subst.
+      8: sep_easy; autorewrite with sepFormula ; rereg; try subst.
+      Focus 8.
+      instantiate (1 := x15).
+
+      Print HintDb core.
+      
+      words.
+      debug auto with contradiction.
+      8: sep_easy; autorewrite with sepFormula ; rereg; try subst.
+      
+      
+      
+
+   sep_firstorder; clear_junk
+      Print Ltac cancel.
+      cancel auto_ext.
+
+      assert (   exists
+     (x18 : A) (x19 x20 : list B) (a0 : ST.settings * smem ->
+                                        PropX W (settings * state)) 
+   (x21 : vals),
+     simplify specs
+       (![^[(Ex buf1 : W,
+              (Ex len1 : W,
+               (Ex cols1 : list (W * W),
+                (Ex bs1 : list B,
+                 sel x21 (Data x0) =*> buf1 *
+                 (sel x21 (Data x0) ^+ $ (4)) =*> len1 *
+                 array (posl cols1) (sel x21 (Data x0) ^+ $ (8)) *
+                 array (lenl cols1)
+                   (sel x21 (Data x0) ^+ $ (8)
+                    ^+ $ (Datatypes.length (Schema (Table x0)) * 4)) *
+                 array8 bs1 buf1 * [|Datatypes.length bs1 = wordToNat len1|] *
+                 [|Datatypes.length cols1 =
+                   Datatypes.length (Schema (Table x0))|] *
+                 [|RelDb.inBounds len1 cols1|] *
+                 [|sel x21 (Data x0) = 0 -> False|] *
+                 [|freeable (sel x21 (Data x0))
+                     (S
+                        (S
+                           (Datatypes.length (Schema (Table x0)) +
+                            Datatypes.length (Schema (Table x0)))))|] *
+                 [|buf1 = 0 -> False|] *
+                 [|freeable8 buf1 (Datatypes.length bs1)|] *
+                 [|sel x21 "matched" =
+                   selN (lenl cols1) (findCol (Schema (Table x0)) col1)|]))))] * 
+          #0] (a, b))
+       (SCons (ST.settings * smem) nil a0 (SNil W (settings * state)))).
+
+      desc.
+      step auto_ext.
+      Print Ltac step.
+
+      assert (   exists
+     (x18 : A) (x19 x20 : list B) (a0 : ST.settings * smem ->
+                                        PropX W (settings * state)) 
+   (x21 : vals),
+     simplify specs
+       (![^[locals ("rp" :: ns) x21 res (Regs b Sp) *
+            (array8 x19 (sel x21 "buf") * array8 x20 (sel x21 "obuf") *
+             [|Datatypes.length x19 = wordToNat (sel x21 "len")|] *
+             [|Datatypes.length x20 = wordToNat (sel x21 "olen")|] *
+             [|inBounds cdatas (sel x21)|] *
+             [|sel x21 "olen" < sel x21 "opos" -> False|] *
+             invPre x18 (sel x21) *
+             cursors (sel x21)
+               (removeCursor (Name (Table x))
+                  (removeCursor (Name (Table x0)) avs)) * 
+             db ts *
+             inv (Address (Table x0)) (Schema (Table x0)) 
+               (sel x21 (Row x0)) (sel x21 (Data x0)) *
+             inv (Address (Table x)) (Schema (Table x)) 
+               (sel x21 (Row x)) (sel x21 (Data x)) *
+             (Ex buf1 : W,
+              (Ex len1 : W,
+               (Ex cols1 : list (W * W),
+                (Ex bs1 : list B,
+                 sel x21 (Data x0) =*> buf1 *
+                 (sel x21 (Data x0) ^+ $ (4)) =*> len1 *
+                 array (posl cols1) (sel x21 (Data x0) ^+ $ (8)) *
+                 array (lenl cols1)
+                   (sel x21 (Data x0) ^+ $ (8)
+                    ^+ $ (Datatypes.length (Schema (Table x0)) * 4)) *
+                 array8 bs1 buf1 * [|Datatypes.length bs1 = wordToNat len1|] *
+                 [|Datatypes.length cols1 =
+                   Datatypes.length (Schema (Table x0))|] *
+                 [|RelDb.inBounds len1 cols1|] *
+                 [|sel x21 (Data x0) = 0 -> False|] *
+                 [|freeable (sel x21 (Data x0))
+                     (S
+                        (S
+                           (Datatypes.length (Schema (Table x0)) +
+                            Datatypes.length (Schema (Table x0)))))|] *
+                 [|buf1 = 0 -> False|] *
+                 [|freeable8 buf1 (Datatypes.length bs1)|] *
+                 [|sel x21 "matched" =
+                   selN (lenl cols1) (findCol (Schema (Table x0)) col1)|])))) *
+             (Ex buf2 : W,
+              (Ex len2 : W,
+               (Ex cols2 : list (W * W),
+                (Ex bs2 : list B,
+                 sel x21 (Data x) =*> buf2 *
+                 (sel x21 (Data x) ^+ $ (4)) =*> len2 *
+                 array (posl cols2) (sel x21 (Data x) ^+ $ (8)) *
+                 array (lenl cols2)
+                   (sel x21 (Data x) ^+ $ (8)
+                    ^+ $ (Datatypes.length (Schema (Table x)) * 4)) *
+                 array8 bs2 buf2 * [|Datatypes.length bs2 = wordToNat len2|] *
+                 [|Datatypes.length cols2 =
+                   Datatypes.length (Schema (Table x))|] *
+                 [|RelDb.inBounds len2 cols2|] *
+                 [|sel x21 (Data x) = 0 -> False|] *
+                 [|freeable (sel x21 (Data x))
+                     (S
+                        (S
+                           (Datatypes.length (Schema (Table x)) +
+                            Datatypes.length (Schema (Table x)))))|] *
+                 [|buf2 = 0 -> False|] *
+                 [|freeable8 buf2 (Datatypes.length bs2)|] *
+                 [|findCol (Schema (Table x)) col2 <
+                   Datatypes.length (lenl cols2)|]%nat)))))] * 
+          #0] (a, b))
+       (SCons (ST.settings * smem) nil a0 (SNil W (settings * state))) /\
+     (exists a1 : ST.settings * state -> PropX W (settings * state),
+        specs (sel x21 "rp") = Some (fun x22 : settings * state => a1 x22) /\
+        (forall x22 : state,
+         interp specs
+           (([|Regs x22 Sp = Regs b Sp|] /\
+             (Ex x23 : vals,
+              (Ex x24 : list B,
+               subst (G := ((settings * state)%type : Type) :: nil)
+                 (subst (G := ((settings * state)%type : Type)
+                   :: ((settings * smem)%type : Type) :: nil)
+                    (![^[locals ("rp" :: ns) x23 res (Regs b Sp) *
+                         (array8 x19 (sel x21 "buf") *
+                          array8 x24 (sel x21 "obuf") *
+                          [|Datatypes.length x24 = Datatypes.length x20|] *
+                          invPost x18 (sel x21) (Regs x22 Rv))] * 
+                       #1] (a, x22)) a0) a1)))%PropX ---> 
+            a1 (a, x22))))).
+
+      desc.
+
+      match goal with
+        | [ _ : context[locals _ ?V _ _] |- _ ] =>
+          instantiate (2 := V)
+      end.
+      descend.
+      step auto_ext.
+
+      assert (interp specs (![ Emp ] (a, b))) by admit; clear H38.
+      clear Hrp Hres H H0 IHxm H5 H6 H7 H8 H9 H10 H11 H12 H13 H29.
+      clear H17 H16 H18 H19 H21 H28 H14 H24 H36 H36 H74 H75 H76 H77 H37
+        H78 H79 H80 H81 H82 H83 H84 H85 H86 H87 H88 H89 H90 H91 H92 H93.
+
+
+      assert (interp specs
+          (![(fun (stn : ST.settings) (sm : smem) => x7 (stn, sm)) *
+             SEP.ST.star
+               (inv (Address (Table x0)) (Schema (Table x0))
+                  (sel x8 (Row x0)) (sel x8 (Data x0)))
+               (SEP.ST.star
+                  (inv (Address (Table x)) (Schema (Table x))
+                     (sel x8 (Row x)) (sel x8 (Data x)))
+                  (SEP.ST.star (db ts)
+                     (SEP.ST.star
+                        (cursors x8
+                           (removeCursor (Name (Table x))
+                              (removeCursor (Name (Table x0)) avs)))
+                        (SEP.ST.star (invPre x4 x8)
+                           (SEP.ST.star (array8 x5 (sel x8 "buf"))
+                              (SEP.ST.star (array8 x6 (sel x8 "obuf"))
+                                 (SEP.ST.star (array8 x14 x17)
+                                    (SEP.ST.star (array8 x10 x13)
+                                       (SEP.ST.star
+                                          (locals ("rp" :: ns)
+                                             (upd
+                                                (upd
+                                                  (upd x8 "matched"
+                                                  (sel x8 (Data x0) ^+ natToW 8))
+                                                  "matched"
+                                                  (sel x8 (Data x0) ^+ natToW 8
+                                                  ^+ 
+                                                  natToW (Datatypes.length
+                                                  (Schema (Table x0)) * 4)%nat))
+                                                "matched"
+                                                (Array.sel 
+                                                  (lenl x15)
+                                                  (findCol
+                                                  (Schema (Table x0)) col1)))
+                                             res (Regs x3 Sp))
+                                          (SEP.ST.star
+                                             (array 
+                                                (posl x15)
+                                                (sel x8 (Data x0) ^+ natToW 8))
+                                             (SEP.ST.star
+                                                (array 
+                                                  (lenl x15)
+                                                  (sel x8 (Data x0) ^+ natToW 8
+                                                  ^+ 
+                                                  natToW (Datatypes.length
+                                                  (Schema (Table x0)) * 4)%nat))
+                                                (SEP.ST.star
+                                                  (array 
+                                                  (posl x11)
+                                                  (sel x8 (Data x) ^+ natToW 8))
+                                                  (SEP.ST.star
+                                                  (array 
+                                                  (lenl x11)
+                                                  (sel x8 (Data x) ^+ natToW 8
+                                                  ^+ 
+                                                  natToW (Datatypes.length
+                                                  (Schema (Table x)) * 4)%nat))
+                                                  (SEP.ST.star
+                                                  (sel x8 (Data x0) =*> x17)
+                                                  (SEP.ST.star
+                                                  ((sel x8 (Data x0) ^+ natToW 4) =*>
+                                                  x16)
+                                                  (SEP.ST.star
+                                                  (sel x8 (Data x) =*> x13)
+                                                  (SEP.ST.star
+                                                  ((sel x8 (Data x) ^+ natToW 4) =*>
+                                                  x12)
+                                                  (SEP.ST.star
+                                                  (SEP.ST.inj
+                                                  [|
+                                                  Datatypes.length x5 =
+                                                  wordToNat (sel x8 "len")|])
+                                                  (SEP.ST.star
+                                                  (SEP.ST.inj
+                                                  [|
+                                                  Datatypes.length x6 =
+                                                  wordToNat (sel x8 "olen")|])
+                                                  (SEP.ST.star
+                                                  (SEP.ST.inj
+                                                  [|inBounds cdatas x8|])
+                                                  (SEP.ST.star
+                                                  (SEP.ST.inj
+                                                  [|
+                                                  sel x8 "opos" <=
+                                                  sel x8 "olen"|])
+                                                  (SEP.ST.star
+                                                  (SEP.ST.inj
+                                                  [|
+                                                  Datatypes.length x14 =
+                                                  wordToNat x16|])
+                                                  (SEP.ST.star
+                                                  (SEP.ST.inj
+                                                  [|
+                                                  Datatypes.length x15 =
+                                                  Datatypes.length
+                                                  (Schema (Table x0))|])
+                                                  (SEP.ST.star
+                                                  (SEP.ST.inj
+                                                  [|RelDb.inBounds x16 x15|])
+                                                  (SEP.ST.star
+                                                  (SEP.ST.inj
+                                                  [|sel x8 (Data x0) <> 0|])
+                                                  (SEP.ST.star
+                                                  (SEP.ST.inj
+                                                  [|
+                                                  freeable 
+                                                  (sel x8 (Data x0))
+                                                  (S
+                                                  (S
+                                                  (Datatypes.length
+                                                  (Schema (Table x0)) +
+                                                  Datatypes.length
+                                                  (Schema (Table x0)))))|])
+                                                  (SEP.ST.star
+                                                  (SEP.ST.inj [|x17 <> 0|])
+                                                  (SEP.ST.star
+                                                  (SEP.ST.inj
+                                                  [|
+                                                  freeable8 x17
+                                                  (Datatypes.length x14)|])
+                                                  (SEP.ST.star
+                                                  (SEP.ST.inj
+                                                  [|
+                                                  findCol 
+                                                  (Schema (Table x0)) col1 <
+                                                  Datatypes.length (lenl x15)|]%PropX%nat)
+                                                  (SEP.ST.star
+                                                  (SEP.ST.inj
+                                                  [|
+                                                  Datatypes.length x10 =
+                                                  wordToNat x12|])
+                                                  (SEP.ST.star
+                                                  (SEP.ST.inj
+                                                  [|
+                                                  Datatypes.length x11 =
+                                                  Datatypes.length
+                                                  (Schema (Table x))|])
+                                                  (SEP.ST.star
+                                                  (SEP.ST.inj
+                                                  [|RelDb.inBounds x12 x11|])
+                                                  (SEP.ST.star
+                                                  (SEP.ST.inj
+                                                  [|sel x8 (Data x) <> 0|])
+                                                  (SEP.ST.star
+                                                  (SEP.ST.inj
+                                                  [|
+                                                  freeable 
+                                                  (sel x8 (Data x))
+                                                  (S
+                                                  (S
+                                                  (Datatypes.length
+                                                  (Schema (Table x)) +
+                                                  Datatypes.length
+                                                  (Schema (Table x)))))|])
+                                                  (SEP.ST.star
+                                                  (SEP.ST.inj [|x13 <> 0|])
+                                                  (SEP.ST.star
+                                                  (SEP.ST.inj
+                                                  [|
+                                                  freeable8 x13
+                                                  (Datatypes.length x10)|])
+                                                  (SEP.ST.inj
+                                                  [|
+                                                  findCol 
+                                                  (Schema (Table x)) col2 <
+                                                  Datatypes.length (lenl x11)|]%PropX%nat)))))))))))))))))))))))))))))))))))))]
+             (a, b))).
+
+      bash.
+      my_descend.
+      eauto.
+      bash.
+      repeat (bash; my_descend); eauto.
+      
+
+
+
 
       step1.
 
